Define theorem 8.1

SimpleTypeSystem.v
@@ -70,5 +70,154 @@ Inductive Typable : TEnv -> Exp -> Types -> Prop :=
                  Typable (TEBind (TEBind C x t') y (TList t')) e3 t ->
                  Typable C (EMatch e1 e2 x y e3) t.
 
+(* Domains (reuesed) *)
+Inductive in_dom : Env -> Var -> Prop :=
+    | Dom_EBind1 : forall (E : Env) (x : Var) (v : Value),
+                   in_dom (EBind E x v) x
+    | Dom_EBind2 : forall (E : Env) (x y : Var) (v : Value),
+                   in_dom E x -> in_dom (EBind E y v) x.
+
+(* Fig 8.3, 8.4 and 8.5 *)
+Inductive Error : Env -> Exp -> Prop :=
+    | E_IfErr1  : forall (E : Env) (e1 e2 e3 : Exp),
+                    not_bool E e1 ->
+                    Error E (EIf e1 e2 e3)
+    | E_IfErr2    : forall (E : Env) (e1 e2 e3 : Exp),
+                    EvalTo E e1 (VBool true) -> Error E e2 ->
+                    Error E (EIf e1 e2 e3)
+    | E_IfErr3    : forall (E : Env) (e1 e2 e3 : Exp),
+                    EvalTo E e1 (VBool false) -> Error E e3 ->
+                    Error E (EIf e1 e2 e3)
+    | E_PlusErr1  : forall (E : Env) (e1 e2 : Exp),
+                    not_int E e1 ->
+                    Error E (EPlus e1 e2)
+    | E_PlusErr2  : forall (E : Env) (e1 e2 : Exp) (i1 : Z),
+                    EvalTo E e1 (VInt i1) -> not_int E e2 ->
+                    Error E (EPlus e1 e2)
+    | E_MinusErr1 : forall (E : Env) (e1 e2 : Exp),
+                    not_int E e1 ->
+                    Error E (EMinus e1 e2)
+    | E_MinusErr2 : forall (E : Env) (e1 e2 : Exp) (i1 : Z),
+                    EvalTo E e1 (VInt i1) -> not_int E e2 ->
+                    Error E (EMinus e1 e2)
+    | E_TimesErr1 : forall (E : Env) (e1 e2 : Exp),
+                    not_int E e1 ->
+                    Error E (ETimes e1 e2)
+    | E_TimesErr2 : forall (E : Env) (e1 e2 : Exp) (i1 : Z),
+                    EvalTo E e1 (VInt i1) -> not_int E e2 ->
+                    Error E (ETimes e1 e2)
+    | E_LtErr1    : forall (E : Env) (e1 e2 : Exp),
+                    not_int E e1 ->
+                    Error E (ELt e1 e2)
+    | E_LtErr2    : forall (E : Env) (e1 e2 : Exp) (i1 : Z),
+                    EvalTo E e1 (VInt i1) -> not_int E e2 ->
+                    Error E (ELt e1 e2)
+    | E_VarErr    : forall (E : Env) (x : Var),
+                    ~ in_dom E x ->
+                    Error E (EVar x)
+    | E_LetErr1   : forall (E : Env) (e1 e2 : Exp) (x : Var),
+                    Error E e1 ->
+                    Error E (ELet x e1 e2)
+    | E_LetErr2   : forall (E : Env) (e1 e2 : Exp) (x : Var) (v1 : Value),
+                    EvalTo E e1 v1 -> Error (EBind E x v1) e2 ->
+                    Error E (ELet x e1 e2)
+    | E_AppErr1   : forall (E : Env) (e1 e2 : Exp),
+                    not_closure E e1 ->
+                    Error E (EApp e1 e2)
+    | E_AppErr2   : forall (E E2 : Env) (e1 e2 e0 : Exp) (x : Var),
+                    EvalTo E e1 (VFun E2 x e0) -> Error E e2 ->
+                    Error E (EApp e1 e2)
+    | E_AppErr3   : forall (E E2 : Env) (e1 e2 e0 : Exp) (x y : Var),
+                    EvalTo E e1 (VRecFun E2 x y e0) -> Error E e2 ->
+                    Error E (EApp e1 e2)
+    | E_AppErr4   : forall (E E2 : Env) (e1 e2 e0 : Exp) (x : Var) (v2 : Value),
+                    EvalTo E e1 (VFun E2 x e0) -> EvalTo E e2 v2 ->
+                    Error (EBind E x v2) e0 ->
+                    Error E (EApp e1 e2)
+    | E_AppErr5   : forall (E E2 : Env) (e1 e2 e0 : Exp)
+                           (x y : Var) (v2 : Value),
+                    EvalTo E e1 (VRecFun E2 x y e0) -> EvalTo E e2 v2 ->
+                    Error (EBind (EBind E x (VRecFun E2 x y e0)) y v2) e0 ->
+                    Error E (EApp e1 e2)
+    | E_LetRecErr : forall (E : Env) (e1 e2 : Exp) (x y : Var),
+                    Error (EBind E x (VRecFun E x y e1)) e2 ->
+                    Error E (ELetRec x y e1 e2)
+    | E_ConsErr1  : forall (E : Env) (e1 e2 : Exp),
+                    Error E e1 ->
+                    Error E (ECons e1 e2)
+    | E_ConsErr2  : forall (E : Env) (e1 e2 : Exp) (v1 : Value),
+                    EvalTo E e1 v1 -> Error E e2 ->
+                    Error E (ECons e1 e2)
+    | E_MatchErr1 : forall (E : Env) (e1 e2 e3 : Exp) (x y : Var),
+                    not_list E e1 ->
+                    Error E (EMatch e1 e2 x y e3)
+    | E_MatchErr2 : forall (E : Env) (e1 e2 e3 : Exp) (x y : Var),
+                    EvalTo E e1 VNil -> Error E e2 ->
+                    Error E (EMatch e1 e2 x y e3)
+    | E_MatchErr3 : forall (E : Env) (e1 e2 e3 : Exp)
+                           (x y : Var) (v1 v2 : Value),
+                    EvalTo E e1 (VCons v1 v2) ->
+                    Error (EBind (EBind E x v1) y v2) e3 ->
+                    Error E (EMatch e1 e2 x y e3)
+    with not_int : Env -> Exp -> Prop :=
+    | NI_Value : forall (E : Env) (e : Exp) (v : Value),
+                 EvalTo E e v -> (forall i : Z, v <> VInt i) ->
+                 not_int E e
+    | NI_Error : forall (E : Env) (e : Exp),
+                 Error E e ->
+                 not_int E e
+    with not_bool : Env -> Exp -> Prop :=
+    | NB_Value : forall (E : Env) (e : Exp) (v : Value),
+                 EvalTo E e v -> (forall b : bool, v <> VBool b) ->
+                 not_bool E e
+    | NB_Error : forall (E : Env) (e : Exp),
+                 Error E e ->
+                 not_bool E e
+    with not_closure : Env -> Exp -> Prop :=
+    | NC_Value : forall (E : Env) (e : Exp) (v : Value),
+                 EvalTo E e v ->
+                 (forall (E0 : Env) (x0 : Var) (e0 : Exp), v <> VFun E0 x0 e0) ->
+                 (forall (E0 : Env) (x0 y0 : Var) (e0 : Exp),
+                  v <> VRecFun E0 x0 y0 e0) ->
+                 not_closure E e
+    | NC_Error : forall (E : Env) (e : Exp),
+                 Error E e ->
+                 not_closure E e
+    with not_list : Env -> Exp -> Prop :=
+    | NL_Value : forall (E : Env) (e : Exp) (v : Value),
+                 EvalTo E e v -> v <> VNil ->
+                 (forall v1 v2 : Value, v <> VCons v1 v2) ->
+                 not_list E e
+    | NL_Error : forall (E : Env) (e : Exp),
+                 Error E e ->
+                 not_list E e.
+
+Inductive halt : Env -> Exp -> Prop :=
+    | H_Value : forall (E : Env) (e : Exp) (v : Value),
+                EvalTo E e v ->
+                halt E e
+    | H_Error : forall (E : Env) (e : Exp),
+                Error E e ->
+                halt E e.
+
+(* Theorem 8.1 *)
+Theorem type_safety_no_error :
+    forall (e : Exp) (t t1 t2 t' : Types) (v : Value),
+    Typable TEEmpty e t -> halt EEmpty e ->
+    (t = TInt ->
+     exists i : Z, EvalTo EEmpty e (VInt i)) /\
+    (t = TBool ->
+     exists b : bool, EvalTo EEmpty e (VBool b)) /\
+    (t = TFun t1 t2 ->
+     exists (E : Env) (x : Var) (e : Exp),
+         EvalTo EEmpty e (VFun E x e) \/
+     exists (E : Env) (x y : Var) (e : Exp),
+         EvalTo EEmpty e (VRecFun E x y e)) /\
+    (t = TList t' ->
+     EvalTo EEmpty e VNil \/
+     exists v1 v2 : Value, EvalTo EEmpty e (VCons v1 v2)).
+Proof.
+Admitted.
+
 End SimpleTypeSystem.
 
